## polyh_4x1a
In this version, we process four elements per iteration.<br>
Our unrolled loop starts at the last element of the array, and our index is reduced by 4 per iteration:

$result = a_{0} +x( a_{1} \ +\ x( a_{2} \ +\ x( ...\ +\ x( a_{n-1} \ +\ xa_{n}) ...)))$

Expending the last four elements:

$result = a_{0} + x( a_{1} \ +\ x( a_{2} + x( ... + x( a_{n-3} \ +\ x( a_{n-2} \ +\ x( a_{n-1} \ +\ xa_{n})))) ...))$<br>
$\qquad= a_{0} +x\left( a_{1} + x\left( a_{2} + x\left( ... + x\left( a_{n-3} \ +\ xa_{n-2} \ +\ x^{2} a_{n-1} \ +\ x^{3} a_{n}\right) ...\right)\right)\right)$

We can continue and expand the next four elements:

$\qquad=\ a_{0} +x\left( ...a_{n-7} \ +\ x\left( a_{n-6} \ +\ x\left( a_{n-5} \ +\ x\left( a_{n-4} \ +\ x\left( a_{n-3} \ +\ xa_{n-2} \ +\ x^{2} a_{n-1} \ +\ x^{3} a_{n}\right)\right)\right)\right) ...\right)$
$\qquad=\ a_{0} +x\left( ...a_{n-7} \ +\ xa_{n-6} \ +\ x^{2} a_{n-5} \ +\ x^{3} a_{n-4} \ +\ x^{4}\left( a_{n-3} \ +\ xa_{n-2} \ +\ x^{2} a_{n-1} \ +\ x^{3} a_{n}\right) ...\right)$

Now, let's define $\displaystyle batch_{i}$ as:

$batch_{i} = xa_{i-3} + xa_{i-2} + x^{2} a_{i-1} + x^{3} a_{i}$

Now:

$result\ =\ a_{0} +x( a_{1} +x\left( ...\ \left( batch_{n-8} +x^{4} *\left( batch_{n-4} +x^{4} *batch_{n}\right) ...\right)\right)$

We'll compute every batch iteration $i$ as defined above and add to the previous batch ($i-4$) multiplied by $x^{4}$:

$iter_{n} = batch_{n}$<br>
$iter_{i} = batch_{i} + x^{4} * iter_{i+4}$

\* We'll add another for loop to iterate the remaining items.

```c
double polyh_4x1a(double a[], double x, long degree)
{
    double x_2 = x * x;
    double x_3 = x_2 * x;
    double x_4 = x_3 * x;
    
    long i;
    double tmp0, tmp1, tmp2, tmp3, tmp_total;
    double result = a[degree];
    for (i = degree - 1; i >= 3; i -=4) {
        // result = a[i-3] + x * (a[i-2] + x * (a[i-1] + x * (a[i] + x * result))); // unrolling (k=4)
        // result = a[i-3] + x * a[i-2] + x_2 * a[i-1] + x_3 * a[i] + x_4 * result; // expanding
        // reassociation:
        tmp0 = x_3 * a[i];
        tmp1 = x_2 * a[i-1];
        tmp2 = x * a[i-2];
        tmp3 = a[i-3];
        tmp_total = (tmp0 + tmp1) + (tmp2 + tmp3);

        result = x_4 * result + tmp_total;
    }

    for (; i >= 0; i--) {
        result = a[i] + x * result;
    }

    return result;
}
```

## polyh_4x4
The challenge here is to come up with a way to have multiple independent accumulators.<br>
As concluded from the previous section:

$result\ =\ a_{0} +x( a_{1} +x\left( ...\ \left( batch_{n-8} +x^{4} *\left( batch_{n-4} +x^{4} * batch_{n}\right) ...\right)\right))$

But:

$batch_{n} = a_{n-3} + xa_{n-2} + x^{2} a_{n-1} + x^{3} a_{n}$<br>
$batch_{n-4} = a_{n-7} + xa_{n-6} + x^{2} a_{n-5} + x^{3} a_{n-4}$<br>
$batch_{n-8} = a_{n-11} + xa_{n-10} + x^{2} a_{n-9} + x^{3} a_{n-8}$<br>
$batch_{n-12} = ...$<br>

So:

$\qquad\ = a_{0} +x( a_{1} +x\left( ...\left( a_{n-11} + xa_{n-10} + x^{2} a_{n-9} + x^{3} a_{n-8}\right) +x^{4} *\left( a_{n-7} + xa_{n-6} + x^{2} a_{n-5} + x^{3} a_{n-4} + x^{4} * a_{n-3} + x^{4} * xa_{n-2} + + x^{4} * x^{2} a_{n-1} + + x^{4} * x^{3} a_{n}\right) ...\right))$

$\qquad\ = a_{0} + x (a_{1} + x ( ... ($<br>
$\qquad\qquad ...\left( a_{n-11} + x^{4} * \left( a_{n-7} + x^{4} * a_{n-3}\right)\right) + ... \left( a_{n-10} + x^{4} * \left( a_{n-6} +x^{4} * xa_{n-2} \right)\right) + ...\left( a_{n-9} + x^{4} * \left( a_{n-5} +x^{4} *x^{2} a_{n-1}\right)\right) + ... \left( a_{n-8} +x^{4} * \left( a_{n-4} + x^{4} * x^{3} a_{n}\right)\right)$<br>
$\qquad\ \ \ )\ ...))$<br>

We were able to convert our accumulation into four independent accumulators:

$result =  ...\left( a_{n-8} +x^{4} *\left( a_{n-4} +x^{4} *x^{3} a_{n}\right)\right)$<br>
$result1 = ...\left( a_{n-9} + x^{4} *\left( a_{n-5} +x^{4} *x^{2} a_{n-1}\right)\right)$<br>
$result2 = ...\left( a_{n-10} + x^{4} *\left( a_{n-6} +x^{4} *xa_{n-2}\right)\right)$<br>
$result3 = ...\left( a_{n-11} \ +x^{4} *\left( a_{n-7} +x^{4} *a_{n-3}\right)\right)$


\* Once again, we add another for loop to iterate the remaining items.

```c
double polyh_4x4(double a[], double x, long degree)
{
    double x_2 = x * x;
    double x_3 = x_2 * x;
    double x_4 = x_3 * x;
    
    long i;
    double result = a[degree];
    double result1 = 0;
    double result2 = 0;
    double result3 = 0;

    if (degree >= 3) {
        result = x_3 * a[degree];
        result1 = x_2 * a[degree-1];
        result2 = x * a[degree-2];
        result3 = a[degree-3];
    }
    
    for (i = degree - 4; i >= 3; i -=4) {
        result  = x_4 * result  + x_3 * a[i];
        result1 = x_4 * result1 + x_2 * a[i-1];
        result2 = x_4 * result2 + x   * a[i-2];
        result3 = x_4 * result3 + a[i-3];
    }

    result = result + result1 + result2 + result3;

    for (; i >= 0; i--) {
        result = a[i] + x * result;
    }

    return result;
}
```

## polyh_8x8

Here we use the same principle as our 4x4 loop unrolling but with 8 accumulators.

```c
double polyh_8x8(double a[], double x, long degree)
{
    double x_2 = x * x;
    double x_3 = x_2 * x;
    double x_4 = x_3 * x;
    double x_5 = x_4 * x;
    double x_6 = x_5 * x;
    double x_7 = x_6 * x;
    double x_8 = x_7 * x;
    
    long i;
    double tmp0, tmp1, tmp2, tmp3, tmp_total;
    double result = a[degree];
    double result1 = 0;
    double result2 = 0;
    double result3 = 0;
    double result4 = 0;
    double result5 = 0;
    double result6 = 0;
    double result7 = 0;

    if (degree >= 7) {
        result = x_7 * a[degree];
        result1 = x_6 * a[degree-1];
        result2 = x_5 * a[degree-2];
        result3 = x_4 * a[degree-3];
        result4 = x_3 * a[degree-4];
        result5 = x_2 * a[degree-5];
        result6 = x * a[degree-6];
        result7 = a[degree-7];
    }
    
    for (i = degree - 8; i >= 8; i -=8) {
        result  = x_8 * result  + x_7 * a[i];
        result1 = x_8 * result1 + x_6 * a[i-1];
        result2 = x_8 * result2 + x_5 * a[i-2];
        result3 = x_8 * result3 + x_4 * a[i-3];
        result4 = x_8 * result4 + x_3 * a[i-4];
        result5 = x_8 * result5 + x_2 * a[i-5];
        result6 = x_8 * result6 + x * a[i-6];
        result7 = x_8 * result7 + a[i-7];
    }

    result = result + result1 + result2 + result3 + result4 + result5 + result6 + result7;

    for (; i >= 0; i--) {
        result = a[i] + x * result;
    }

    return result;
}
```


## Performance testing

The result I got on my M1 Pro machine:
```

> clang -o 18 18.c && ./18
 [polyh]: 		4788 ticks
 [polyh_4x1a]: 		1042 ticks
 [polyh_4x4]: 		961 ticks
 [polyh_8x8]: 		768 ticks
```
6.2 times faster!
<br><br>


```
> clang -o 18 -arch x86_64 18.c && ./18
 [polyh]: 		5121 ticks
 [polyh_4x1a]: 		1240 ticks
 [polyh_4x4]: 		1225 ticks
 [polyh_8x8]: 		761 ticks

```
6.7 times faster!
